\subsection{Chain rule}
$$f: \mathbb{R}^2 \to \mathbb{R}$$
$$g: \mathbb{R} \to \mathbb{R}$$
$$h: \mathbb{R} \to \mathbb{R}^2$$

\paragraph{$g \circ f$} Suppose $f$ has partial derivatives and $g$ is differentiable:
$$(g\circ f)(x,y) = g(f(,x,y))$$ 
$$\frac{\partial}{\partial x} (g\circ f)(x,y) = g^\prime (f(x,y)) \frac{\partial x}{\partial y}(x,y)$$
\paragraph{$f \circ h$} 
$$h:[a,b]\to \mathbb{R}^2 \quad h(t) = \left(h_1(t), h_2(t)\right) = \left(x(t), y(t)\right)$$
\subparagraph{Definition} Such $h$, if continuous (i.e. $h_i$ is continuous) is called track.

Let $f$ differentiable on interval $D$ and $h$ - track in $D$ such that $x(t)$, $y(t)$ are differentiable. Denote $F(t) = f(x(t), y(t))$. Then $F$ is differentiable and 
$$\frac{dF}{dt}= \frac{\partial f}{\partial x}(x(t), y(t)) \cdot \frac{dx}{dt}(t) + \frac{\partial f}{\partial y}(x(t), y(t)) \cdot \frac{dy}{dt}(t) = \nabla f \cdot h^\prime$$
$$h^\prime (t) = \left(x^\prime(t), y^\prime(t)\right)$$
\subparagraph{Proof}
Let $t\in [a,b]$. Define 
$$\Delta x = x\left(t+\Delta t\right) - x(t)$$ 
$$\Delta y = y\left(t+\Delta t\right) - y(t)$$ 
From continuousness and differentiability of $x$ and $y$;
$$\Delta x, \Delta y \stackrel{\Delta t \to 0}{\to} 0$$
$$\frac{\Delta x}{\Delta t} \stackrel{\Delta t \to 0}{\to} x^\prime(t)$$ 
$$\frac{\Delta y}{\Delta t} \stackrel{\Delta t \to 0}{\to} y^\prime(t)$$ 
From differentiability of $f$:
\begin{align*}
\Delta F = F(t+\Delta t) - F(t) = f(x(t)+\Delta x, y(t)+\Delta y) - f(x(t),y(t)) =\\= \frac{\partial f}{\partial x}(x(t), y(t)) \Delta x+\frac{\partial f}{\partial y}(x(t), y(t)) \Delta y + \alpha (\Delta x, \Delta y)\Delta x + \beta (\Delta x, Delta y)\Delta y\end{align*}
$$\alpha (\Delta x, \Delta y) \stackrel{\Delta x, \Delta y \to 0}{\to} 0 \Rightarrow \alpha (\Delta x, \Delta y) \stackrel{\Delta t \to 0}{\to} 0$$
$$\beta (\Delta x, \Delta y) \stackrel{\Delta x, \Delta y \to 0}{\to} 0 \Rightarrow \beta (\Delta x, \Delta y) \stackrel{\Delta t \to 0}{\to} 0$$
$$\frac{\Delta F}{\Delta t} = \frac{\partial f}{\partial x} \cdot \frac{\Delta x}{\Delta t}+\frac{\partial f}{\partial y} \cdot \frac{\Delta y}{\Delta t} + \alpha (\Delta x, \Delta y)\frac{\Delta x}{\Delta t} + \beta (\Delta x, Delta y)\cdot \frac{\Delta y}{\Delta t}\stackrel{\Delta t \to 0}{\to} \frac{\partial f}{\partial x} \cdot x^\prime +\frac{\partial f}{\partial y} \cdot y^\prime $$
\paragraph{Example}
$h(t) = (e^t, \cos t)$ and $f(x,y) xy$.
$$F(t) = e^t\cos^t$$
$$\frac{\partial f}{\partial x} = y$$
$$\frac{\partial f}{\partial y} = x$$
$$x^\prime (t) = e^t$$
$$y^\prime (t) = -\sin t$$
$$F^\prime (t) = ye^t + x(-\sin t) = e^t\cos t -e^t \sin t$$
\paragraph{Fact} If $D$ is interval (open and connected) then for any $x^0, x^1 \in D$ exists track $\gamma: [0,1] \to D$ such that $\gamma(0) = x^0$, $\gamma(1) = x^1$ and $\gamma$ is derivable.
\paragraph{Conclusion} If $f$ has  partial derivatives in interval $D$ such that

$$\frac{\partial f}{\partial y} = \frac{\partial f}{\partial x} \equiv 0$$
then $f$ is constant.
\paragraph{Proof}
$\forall x^0, y^1 \in D \: \exists \gamma: [0,1] \to D$ derivable such that $\gamma(0)=x^0$ and $\gamma(1)=x^1$.
$$F(t) = f\circ \gamma \Rightarrow F^\prime = \nabla f \cdot \gamma^\prime$$
$$f(x^0) = F(\gamma(0)) = F(\gamma(1)) = f(x^1)$$
\subsection{High order derivatives}
Denote
$$\frac{\partial }{\partial x} \left( \frac{\partial f}{\partial x} \right) = \frac{\partial^2 f}{\partial x^2} = f_{xx}$$
$$\frac{\partial }{\partial y} \left( \frac{\partial f}{\partial x} \right) = \frac{\partial^2 f}{\partial y \partial x} = f_{xy}$$
\paragraph{Example}
$$f(x,y) = e^{xy}\cos y$$
$$\frac{\partial f}{\partial x} = ye^{xy}\cos y$$
$$\frac{\partial f}{\partial y} = xe^{xy}\cos y - e^{xy}\sin y $$
$$\frac{\partial^2 f}{\partial x^2} = y^2e^{xy}\cos y$$
$$\frac{\partial^2 f}{\partial y\partial x} = e^{xy}\cos y + xye^{xy}\cos y - ye^{xy}\sin y$$
$$\frac{\partial^2 f}{\partial x\partial y} = e^{xy}\cos y + xye^{xy}\cos y - ye^{xy}\sin y$$

\paragraph{Sentence}
If $f$ defined on open set $D$ and both mixed derivatives exist and continuous, they are equal.
\subparagraph{Proof}
Choose $(x_0, y_0) \in D$, such that rectangle with sides of $\Delta x$, $\Delta y$ is fully inside $D$.
Denote
$$S(\Delta x, \Delta y) = \big[ f(x_0+\Delta x, y_0 + \Delta y) - f(x_0+\Delta x, y_0) \big] - \big[ f(x_0, y_0 + \Delta y) - f(x_0, y_0) \big] = g(x_0+\Delta x) - g(x)$$
where $g(x) = f(x, y_0 + \Delta y) - f(x, y_0)$
With Lagrange on $g$ ($0 <\theta < 1$):
$$S(\Delta x, \Delta y) = g^\prime (x+\theta \Delta x) \Delta x = \big[\frac{\partial f}{\partial x}(x_0+\theta \Delta x, y_0+\Delta y) - \frac{\partial f}{\partial x}(x_0+\theta \Delta x, y_0)\big]\Delta x$$
Once again by Lagrange
$$S(\Delta x, \Delta y) = g^\prime (x+\theta \Delta x) \Delta x = \frac{\partial f}{\partial y \partial x}(x_0+\theta \Delta x, y_0+\theta_1\Delta y)\Delta x\Delta y$$
$$\frac{S(\Delta x, \Delta y)}{\Delta x \Delta y} = \frac{\partial f}{\partial y \partial x}(x_0+\theta \Delta x, y_0+\theta_1\Delta y) \stackrel{\Delta x, \Delta y \to 0}{\to} \frac{\partial f}{\partial y \partial x}(x_0, y_0)$$
\subsection{Integrals with parameter}
\paragraph{Sentence} Let $f$ defined on $[a,b] \times [\alpha, \beta]$ and continuous there. Define
$$F(s,t,u) = \int_s^t f(x,u) dx$$
Then $F$ is continuous on $[a,b] \times [a,b] \times [\alpha, \beta]$.
\subparagraph{Proof}
Choose $\epsilon > 0 $. Since $f$ is continuous on closed finite rectangle, it's uniformly continuous. Then $\exists \delta >0 $ such that if $d(x^0,x^1) < \delta$ then
$$\left|  f(x^0)-f(x^1)\right| < \frac{\epsilon}{b-a}$$
Choose $s_0$, $t_0$, $u_0$.
Let $M$ such that $$\forall (x,y) \in [a,b] \times [\alpha, \beta] \: |f(x,y)| \leq M$$
Choose $s$,$t$,$u$ such that
$|u-u_0| < \delta$, 
$|t-t_0| < \frac{\epsilon}{M}$, 
$|s-s_0| < \frac{\epsilon}{M}$. 

Let's show that 
$$\left|F(s,t,u)-F(s_0,t_0,u_0)\right| < 3\epsilon$$

\begin{align*}
\left|F(s,t,u)-F(s_0,t_0,u_0)\right| = \left| \int_s^t f(x,u) dx - \int_{s_0}^{t_0} f(x,u_0) dx\right| \leq \left| \int_s^t f(x,u_0) dx - \int_{s_0}^{t_0} f(x,u_0) dx\right|+\left| \int_s^t f(x,u) dx - \int_{s}^{t} f(x,u_0) dx\right| \leq\\\leq  \left| \int_{t_0}^t f(x,u_0) dx \pm \int_{s_0}^{s} f(x,u_0) dx\right|+\left| \int_s^t f(x,u) dx - \int_{s}^{t} f(x,u_0) dx\right| \leq\\\leq \left| \int_{t_0}^t \left|f(x,u_0)\right| dx \right| + \left|  \int_{s_0}^{s} \left|f(x,u_0)\right| dx\right|+\left| \int_s^t f(x,u) dx - \int_{s}^{t} f(x,u_0) dx\right| \leq\\\leq \left| (t-t_0)M \right| + \left|  (s-s_0)M\right|+\left| \int_s^t f(x,u) dx - \int_{s}^{t} f(x,u_0) dx\right| \leq 2\epsilon +\int_s^t\underbrace{\left|  f(x,u) - f(x,u_0)\right|}_{ \leq \frac{\epsilon}{b-a}} dx \leq 2\epsilon +(t-s)\frac{\epsilon}{b-a} \leq 3\epsilon 
\end{align*}
\paragraph{Sentence}
Let $f$ defined on $[a,b] \times [\alpha, \beta]$ such that $\frac{\partial f}{\partial y}$ and both $f$ and $\frac{\partial f}{\partial y}$ are continuous. Define
$$F(u) = \int_a^b f(x,u) dx$$
Then $F$ is derivable on $[a,b]$ and
$$F^\prime (u) = \int_a^b \frac{\partial }{\partial y}f(x,u) dx$$
\subparagraph{Proof}
By Lagrange($0<\theta < 1$)
$$\Delta F = F(u+\Delta u) - F(u) = \int_a^b \big[ f(x,u+\Delta u) - f(x,u) \big]dx = \int_a^b \frac{\partial f}{\partial y}(x, u+\theta \Delta u) \Delta u dx$$
$$\frac{\Delta F}{\Delta u} = \int_a^b \frac{\partial f}{\partial y}(x, u+\theta \Delta u) dx \stackrel{\Delta u \to 0}{\to} \int_a^b \frac{\partial f}{\partial y} (x,y) dx$$
\paragraph{Sentence}
Let $f$ defined on $[a,b] \times [\alpha, \beta]$ such that $\frac{\partial f}{\partial y}$ and both $f$ and $\frac{\partial f}{\partial y}$ are continuous. Define
$$F(s,t,u) = \int_s^t f(x,u) dx$$
Then all partial derivatives of $F$ exist and continuous, thus, $F$ is differentiable on $[a,b]$.
