\paragraph{Example}
$D$ is an triangle between $(0,0)$, $(1,1)$ and $(1,0)$
and 
$$f(x,y) = \begin{cases}
\frac{1}{x-y}&x\neq y\\0&x=y
\end{cases}$$
Define
$$D_n = \left\{ (x,y): \frac{1}{n}\leq x\leq 1, 0\leq y\leq x-\frac{1}{n} \right\}$$
\begin{align*}
\iint\limits_{D_n} \frac{1}{x-y} = \int_{\frac{1}{n}}^{1}\int_0^{x-\frac{1}{n}}\frac{1}{x-y}dydx = \int_{\frac{1}{n}}^{1} \left[ -\ln(x-y) \right]_0^{x-\frac{1}{n}} dx = \int_{\frac{1}{n}}^{1} -\ln \frac{1}{n} + \ln x dx = \int_{\frac{1}{n}}^{1} \ln n + \ln x dx =\\= \left[ x\ln n + \left( x\ln x - x \right)\right]_{\frac{1}{n}}^{1} = (1-\frac{1}{n})\ln n - 1 + \frac{1}{n} \ln n + \frac{1}{n} = \ln n - (1-\frac{1}{n})
\end{align*}
\paragraph{Convolution}
$f,g: [0, \infty) \to \mathbb{R}$ continuous and $\int_0^\infty |f| dx < \infty $, $\int_0^\infty |g| dx < \infty$ $\forall x \geq 0$ we can define convolution:
$$(f \ast g) (x) = \int_0^x f(t)g(x-t) dt$$
\paragraph{Claim}
$$\int_0^\infty (f \ast g) dx = \int_0^\infty f  \int_0^\infty g$$
\subparagraph{Proof}
$$\int_0^\infty f \int_0^\infty g = \lim_{n \to \infty} \int_0^n f(t) dt \int_0^n g(u)  du$$
Define $s=u+t$
$$\lim_{n \to \infty} \int_0^n f(t) dt \int_0^n g(u)  du = \lim_{n \to \infty} \int_0^n f(t) \int_t^{n+t} g(s-t)  ds dt = \lim_{n \to \infty} \int_0^n\int_t^{n+t} f(t)  g(s-t)  ds dt$$

Define $D = \left\{ (t,s): s \geq t \right\}$
$$\lim_{n \to \infty} \int_0^n\int_t^{n+t} f(t)  g(s-t)  ds dt= \lim \iint\limits_{D_n} f(t)g(s-t) $$
Define $A_n$ as a triangle between $(0,0)$, $(0,n)$ and $(n,n)$. If $ f(t)  g(s-t) $ is integrable we can replace $D_n$ by $A_n$. 
$$\lim \iint\limits_{D_n} f(t)g(s-t) = \lim_{n \to \infty} \iint\limits_{A_n} f(t)g(s-t) = \lim_{n \to \infty} \int_0^n \int_0^s f(t)g(s-t) dt ds = \lim_{n \to \infty} \int_0^n (f\ast g)(s) ds = \int_0^\infty (f\ast g)(s) ds$$
Now we need to show that $ f(t)  g(s-t) $ is integrable. It's true iff $ |f(t)  g(s-t)|$ is integrable. We can show it by proofing that
$\lim_{n \to \infty} \iint\limits_{D_n} |f(t)g(s-t)|$ exists and finite.

By repeating te calculation we can get
$$\infty > \int_0^\infty |f| \int_0^\infty |g| = \dots = \lim \iint\limits_{D_n} |f(t)g(s-t)|$$
\paragraph{Note}
Laplace transform: $$L(f)(x) = \int_0^\infty f(t) e^{-xt} dt$$
It can be shown that
$$L(f\ast g) = L(f)L(g)$$